dovetailn vs dovetail

Computability/Constructions/Dovetail.lean
@@ -10,19 +10,19 @@ Given a code `c`, `dovetail c` gives the code to the function which, on input n,
 returns `y` s.t. `[c](n,y)=0`.
 -/
 
-@[irreducible] def dovetail (c:Code) : Code :=
+def dovetailn (c:Code) : Code :=
   c_rfind $
   c_if_eq'.comp₂
   (c_evaln.comp₃ (pair left (left.comp right)) (c_const c) (right.comp right))
   (c_const 1)
 
-theorem dovetail_ev_0 (h:(eval O (dovetail c) x).Dom) :
-let dvt := (eval O (dovetail c) x).get h
+theorem dovetailn_ev_0 (h:(eval O (dovetailn c) x).Dom) :
+let dvt := (eval O (dovetailn c) x).get h
 evaln O dvt.r c (Nat.pair x (dvt.l))=Option.some 0 := by
   extract_lets; expose_names
-  have dvtrw : (eval O (dovetail c) x).get h = dvt := rfl
+  have dvtrw : (eval O (dovetailn c) x).get h = dvt := rfl
 
-  unfold dovetail at h dvtrw
+  unfold dovetailn at h dvtrw
 
   have := Part.get_mem h
   rw [dvtrw] at this
@@ -35,16 +35,16 @@ evaln O dvt.r c (Nat.pair x (dvt.l))=Option.some 0 := by
   have := Part.eq_some_iff.mpr h4; clear h4
   simp [o2n] at this
   exact Encodable.encode_inj.mp this
-theorem dovetail_ev_0' (h:(eval O (dovetail c) x).Dom) :
-let dvt := (eval O (dovetail c) x).get h
+theorem dovetailn_ev_0' (h:(eval O (dovetailn c) x).Dom) :
+let dvt := (eval O (dovetailn c) x).get h
 eval O c (Nat.pair x (dvt.l))=Part.some 0 := by
-  have := dovetail_ev_0 h
+  have := dovetailn_ev_0 h
   extract_lets
   expose_names
   extract_lets at this
   exact Part.eq_some_iff.mpr (evaln_sound this)
 
-theorem dovetail_ev_1' : eval O (dovetail c) x=Part.none ↔ ∀ s y, evaln O s c (Nat.pair x y)≠Option.some 0 := by
+theorem dovetailn_ev_1' : eval O (dovetailn c) x=Part.none ↔ ∀ s y, evaln O s c (Nat.pair x y)≠Option.some 0 := by
   constructor
   ·
     contrapose
@@ -53,7 +53,7 @@ theorem dovetail_ev_1' : eval O (dovetail c) x=Part.none ↔ ∀ s y, evaln O s 
     intro h
     apply Part.not_none_iff_dom.mpr
 
-    unfold dovetail
+    unfold dovetailn
     simp only [c_rfind_prop]
     simp only [comp₂, comp₃] -- without this theres a recursion depth error. why?
     simp []
@@ -77,14 +77,14 @@ theorem dovetail_ev_1' : eval O (dovetail c) x=Part.none ↔ ∀ s y, evaln O s 
     intro h
     simp
     have hh := Part.not_none_iff_dom.mp h
-    have := dovetail_ev_0 hh
+    have := dovetailn_ev_0 hh
 
     aesop? says
       apply Exists.intro
       apply Exists.intro
       exact this
 
-theorem dovetail_ev_1_aux : (∀ s y, evaln O s c (Nat.pair x y)≠Option.some 0) ↔ ∀ y, eval O c (Nat.pair x y)≠Part.some 0 := by
+theorem dovetailn_ev_1_aux : (∀ s y, evaln O s c (Nat.pair x y)≠Option.some 0) ↔ ∀ y, eval O c (Nat.pair x y)≠Part.some 0 := by
 
   constructor
   contrapose
@@ -101,12 +101,47 @@ theorem dovetail_ev_1_aux : (∀ s y, evaln O s c (Nat.pair x y)≠Option.some 0
   use y
   exact Part.eq_some_iff.mpr (evaln_sound h)
 
-theorem dovetail_ev_1 : eval O (dovetail c) x=Part.none ↔ ∀ y, eval O c (Nat.pair x y)≠Part.some 0 := by
-  exact Iff.trans dovetail_ev_1' dovetail_ev_1_aux
-theorem dovetail_ev_2 : (eval O (dovetail c) x).Dom ↔ ∃ y, eval O c (Nat.pair x y)=Part.some 0 := by
-  have := (@dovetail_ev_1 O c x).not
+theorem dovetailn_ev_1 : eval O (dovetailn c) x=Part.none ↔ ∀ y, eval O c (Nat.pair x y)≠Part.some 0 := by
+  exact Iff.trans dovetailn_ev_1' dovetailn_ev_1_aux
+theorem dovetailn_ev_2 : (eval O (dovetailn c) x).Dom ↔ ∃ y, eval O c (Nat.pair x y)=Part.some 0 := by
+  have := (@dovetailn_ev_1 O c x).not
   simp at this
   exact Iff.trans (Iff.symm Part.not_none_iff_dom) this
 
 
+
+
+
+def dovetail (c:Code) : Code := left.comp (dovetailn c)
+
+theorem dovetail_dom_iff_dovetailn_dom : (eval O (dovetail c) x).Dom ↔ (eval O (dovetailn c) x).Dom := by
+  simp [dovetail,eval]
+theorem dovetail_none_iff_dovetailn_none : (eval O (dovetail c) x) = Part.none ↔ (eval O (dovetailn c) x) = Part.none := by
+  apply not_iff_not.mp
+  simp [not_none_iff_dom]
+  exact dovetail_dom_iff_dovetailn_dom
+theorem dovetail_ev_0 (h:(eval O (dovetail c) x).Dom) :
+let dvt := (eval O (dovetail c) x).get h
+eval O c (Nat.pair x (dvt))=Part.some 0 := by
+  -- sorry
+  have : (eval O (dovetailn c) x).Dom := by
+    exact dovetail_dom_iff_dovetailn_dom.mp h
+  have main := dovetailn_ev_0' this
+  extract_lets
+  extract_lets at main
+  expose_names
+
+  have : dvt = dvt_1.l := by simp [dvt_1,dvt,dovetail, eval, Part.Dom.bind this]
+  rw [this]
+  exact main
+
+theorem dovetail_ev_1' : eval O (dovetail c) x=Part.none ↔ ∀ s y, evaln O s c (Nat.pair x y)≠Option.some 0 := by
+  simp [dovetail_none_iff_dovetailn_none]
+  exact dovetailn_ev_1'
+theorem dovetail_ev_1 : eval O (dovetail c) x=Part.none ↔ ∀ y, eval O c (Nat.pair x y)≠Part.some 0 := by
+  exact Iff.trans dovetail_ev_1' dovetailn_ev_1_aux
+theorem dovetail_ev_2 : (eval O (dovetail c) x).Dom ↔ ∃ y, eval O c (Nat.pair x y)=Part.some 0 := by
+  have := (@dovetail_ev_1 O c x).not
+  simp at this
+  exact Iff.trans (Iff.symm Part.not_none_iff_dom) this
 end Computability.Code
